union 3

lib/Marshalling/UnionMarshalling.i.dfy
@@ -2,14 +2,14 @@ include "MarshalledAccessors.i.dfy"
 // include "../Base/sequences.i.dfy"
 
 abstract module Union2Marshalling refines Marshalling {
-  import LeftMarshalling : Marshalling
-  import RightMarshalling : Marshalling
+  import CaseMarshalling0 : Marshalling
+  import CaseMarshalling1 : Marshalling
   import TagMarshalling : IntegerMarshalling
   // import Sequences
 
   datatype UnionType = 
-    | Left(l : LeftMarshalling.UnmarshalledType)
-    | Right(r: RightMarshalling.UnmarshalledType)
+    | Left(l : CaseMarshalling0.UnmarshalledType)
+    | Right(r: CaseMarshalling1.UnmarshalledType)
 
   type UnmarshalledType = UnionType
 
@@ -27,8 +27,8 @@ abstract module Union2Marshalling refines Marshalling {
     && TagMarshalling.parsable(data[..tagEnd])
     && TagMarshalling.Int.fitsInUint64(TagMarshalling.parse(data[..tagEnd]))
     && var tag := TagMarshalling.Int.toInt(TagMarshalling.parse(data[..tagEnd]));
-    (if tag == 0 then LeftMarshalling.parsable(data[tagEnd..])
-        else RightMarshalling.parsable(data[tagEnd..]))
+    (if tag == 0 then CaseMarshalling0.parsable(data[tagEnd..])
+        else CaseMarshalling1.parsable(data[tagEnd..]))
   }
 
   function parse(data: mseq<byte>) : UnmarshalledType
@@ -36,8 +36,8 @@ abstract module Union2Marshalling refines Marshalling {
     var tagEnd := getTagEnd() as int;
     var tag := TagMarshalling.Int.toInt(TagMarshalling.parse(data[..tagEnd]));
 
-    if tag == 0 then Left(LeftMarshalling.parse(data[tagEnd..]))
-      else Right(RightMarshalling.parse(data[tagEnd..]))
+    if tag == 0 then Left(CaseMarshalling0.parse(data[tagEnd..]))
+      else Right(CaseMarshalling1.parse(data[tagEnd..]))
   }
 
   method TryParse(data: mseq<byte>) returns (ovalue: Option<UnmarshalledType>)
@@ -62,12 +62,12 @@ abstract module Union2Marshalling refines Marshalling {
     ovalue := None;
 
     if tag == 0 {
-      var leftOvalue := LeftMarshalling.TryParse(data[tagEnd..]);
+      var leftOvalue := CaseMarshalling0.TryParse(data[tagEnd..]);
       if leftOvalue.Some? {
         ovalue := Some(Left(leftOvalue.value));
       }
     } else {
-      var rightOvalue := RightMarshalling.TryParse(data[tagEnd..]);
+      var rightOvalue := CaseMarshalling1.TryParse(data[tagEnd..]);
       if rightOvalue.Some? {
         ovalue := Some(Right(rightOvalue.value));
       }
@@ -96,9 +96,9 @@ abstract module Union2Marshalling refines Marshalling {
     var tag := TagMarshalling.Int.toUint64(tagOvalue.value);
 
     if tag == 0 {
-      p := LeftMarshalling.Parsable(data[tagEnd..]);
+      p := CaseMarshalling0.Parsable(data[tagEnd..]);
     } else {
-      p := RightMarshalling.Parsable(data[tagEnd..]);
+      p := CaseMarshalling1.Parsable(data[tagEnd..]);
     }
   }
 
@@ -109,10 +109,10 @@ abstract module Union2Marshalling refines Marshalling {
     var tag := TagMarshalling.Int.toUint64(tagOvalue.value);
 
     if tag == 0 {
-      var leftValue := LeftMarshalling.Parse(data[tagEnd..]);
+      var leftValue := CaseMarshalling0.Parse(data[tagEnd..]);
       value := Left(leftValue);
     } else {
-      var rightValue := RightMarshalling.Parse(data[tagEnd..]);
+      var rightValue := CaseMarshalling1.Parse(data[tagEnd..]);
       value := Right(rightValue);
     }
   }
@@ -121,8 +121,8 @@ abstract module Union2Marshalling refines Marshalling {
   {
     && TagMarshalling.Int.MinValue() <= 0 < 1 < TagMarshalling.Int.UpperBound()
     && match value {
-      case Left(leftValue) => LeftMarshalling.marshallable(leftValue)
-      case Right(rightValue) => RightMarshalling.marshallable(rightValue)
+      case Left(leftValue) => CaseMarshalling0.marshallable(leftValue)
+      case Right(rightValue) => CaseMarshalling1.marshallable(rightValue)
     }
   }
 
@@ -130,8 +130,8 @@ abstract module Union2Marshalling refines Marshalling {
   {
     var tagEnd := getTagEnd();
     match value {
-      case Left(leftValue) => tagEnd as nat + LeftMarshalling.size(leftValue)
-      case Right(rightValue) => tagEnd as nat + RightMarshalling.size(rightValue)
+      case Left(leftValue) => tagEnd as nat + CaseMarshalling0.size(leftValue)
+      case Right(rightValue) => tagEnd as nat + CaseMarshalling1.size(rightValue)
     }
   }
 
@@ -140,11 +140,11 @@ abstract module Union2Marshalling refines Marshalling {
     sz := getTagEnd();
     match value
     case Left(leftValue) => {
-      var leftSize := LeftMarshalling.Size(leftValue);
+      var leftSize := CaseMarshalling0.Size(leftValue);
       sz := sz + leftSize;
     }
     case Right(rightValue) => {
-      var rightSize := RightMarshalling.Size(rightValue);
+      var rightSize := CaseMarshalling1.Size(rightValue);
       sz := sz + rightSize;
     }
   }
@@ -158,7 +158,7 @@ abstract module Union2Marshalling refines Marshalling {
     case Left(leftValue) => {
       newdata, end := TagMarshalling.Marshall(TagMarshalling.Int.fromUint64(0), data, start);
       ghost var newdata1 :seq<byte>, end1 := newdata, end;
-      newdata, end := LeftMarshalling.Marshall(leftValue, newdata, end);
+      newdata, end := CaseMarshalling0.Marshall(leftValue, newdata, end);
 
       assert newdata1[start..end1] == newdata[start..end1];
       ghost var tag := TagMarshalling.Int.toInt(TagMarshalling.parse(newdata[start..end1]));
@@ -170,12 +170,225 @@ abstract module Union2Marshalling refines Marshalling {
     case Right(rightValue) => {
       newdata, end := TagMarshalling.Marshall(TagMarshalling.Int.fromUint64(1), data, start);
       ghost var newdata1 :seq<byte>, end1 := newdata, end;
-      newdata, end := RightMarshalling.Marshall(rightValue, newdata, end);
+      newdata, end := CaseMarshalling1.Marshall(rightValue, newdata, end);
   
       assert newdata1[start..end1] == newdata[start..end1];
       ghost var tag := TagMarshalling.Int.toInt(TagMarshalling.parse(newdata[start..end1]));
       TagMarshalling.Int.fromtoInverses();
       assert tag == 1;
+
+      assert newdata[start..end][..tagEnd] == newdata[start..end1];
+    }
+  }
+}
+
+
+abstract module Union3Marshalling refines Marshalling {
+  import CaseMarshalling0 : Marshalling
+  import CaseMarshalling1 : Marshalling
+  import CaseMarshalling2 : Marshalling
+  import TagMarshalling : IntegerMarshalling
+  // import Sequences
+
+  datatype UnionType = 
+    | Case0(c0: CaseMarshalling0.UnmarshalledType)
+    | Case1(c1: CaseMarshalling1.UnmarshalledType)
+    | Case2(c2: CaseMarshalling2.UnmarshalledType)
+
+  type UnmarshalledType = UnionType
+
+  type TagType = TagMarshalling.UnmarshalledType
+
+  function method getTagEnd(): uint64
+  {
+    TagMarshalling.Int.Size() as uint64
+  }
+
+  predicate parsable(data: mseq<byte>)
+  {
+    var tagEnd := getTagEnd() as int;
+    && |data| >= tagEnd
+    && TagMarshalling.parsable(data[..tagEnd])
+    && TagMarshalling.Int.fitsInUint64(TagMarshalling.parse(data[..tagEnd]))
+    && var tag := TagMarshalling.Int.toInt(TagMarshalling.parse(data[..tagEnd]));
+    (if tag == 0 then CaseMarshalling0.parsable(data[tagEnd..])
+      else if tag == 1 then CaseMarshalling1.parsable(data[tagEnd..])
+      else CaseMarshalling2.parsable(data[tagEnd..]))
+  }
+
+  function parse(data: mseq<byte>) : UnmarshalledType
+  {
+    var tagEnd := getTagEnd() as int;
+    var tag := TagMarshalling.Int.toInt(TagMarshalling.parse(data[..tagEnd]));
+
+    if tag == 0 then Case0(CaseMarshalling0.parse(data[tagEnd..]))
+      else if tag == 1 then Case1(CaseMarshalling1.parse(data[tagEnd..]))
+      else Case2(CaseMarshalling2.parse(data[tagEnd..]))
+  }
+
+  method TryParse(data: mseq<byte>) returns (ovalue: Option<UnmarshalledType>)
+  {
+    var tagEnd := getTagEnd();
+
+    if tagEnd > |data| as uint64 {
+      return None;
+    }
+
+    var tagOvalue := TagMarshalling.TryParse(data[..tagEnd]);
+    
+    if tagOvalue.None? {
+      return None;
+    }
+
+    if !TagMarshalling.Int.fitsInUint64(tagOvalue.value) {
+      return None;
+    }
+
+    var tag := TagMarshalling.Int.toUint64(tagOvalue.value);
+    ovalue := None;
+
+    if tag == 0 {
+      var valueOpt := CaseMarshalling0.TryParse(data[tagEnd..]);
+      if valueOpt.Some? {
+        ovalue := Some(Case0(valueOpt.value));
+      }
+    } else if tag == 1 {
+      var valueOpt := CaseMarshalling1.TryParse(data[tagEnd..]);
+      if valueOpt.Some? {
+        ovalue := Some(Case1(valueOpt.value));
+      }
+    } else {
+      var valueOpt := CaseMarshalling2.TryParse(data[tagEnd..]);
+      if valueOpt.Some? {
+        ovalue := Some(Case2(valueOpt.value));
+      }
+    }
+  }
+
+  method Parsable(data: mseq<byte>) returns (p: bool)
+  {
+    var tagEnd := getTagEnd();
+
+    if tagEnd > |data| as uint64 {
+      return false;
+    }
+
+    var tagOvalue := TagMarshalling.TryParse(data[..tagEnd]);
+    
+    if tagOvalue.None? {
+      return false;
+    }
+
+    if !TagMarshalling.Int.fitsInUint64(tagOvalue.value) {
+      return false;
+    }
+
+    var tag := TagMarshalling.Int.toUint64(tagOvalue.value);
+
+    if tag == 0 {
+      p := CaseMarshalling0.Parsable(data[tagEnd..]);
+    } else if tag == 1{
+      p := CaseMarshalling1.Parsable(data[tagEnd..]);
+    } else {
+      p := CaseMarshalling2.Parsable(data[tagEnd..]);
+    }
+  }
+
+  method Parse(data: mseq<byte>) returns (value: UnmarshalledType)
+  {
+    var tagEnd := getTagEnd();
+    var tagOvalue := TagMarshalling.TryParse(data[..tagEnd]);
+    var tag := TagMarshalling.Int.toUint64(tagOvalue.value);
+
+    if tag == 0 {
+      var val := CaseMarshalling0.Parse(data[tagEnd..]);
+      value := Case0(val);
+    } else if tag == 1 {
+      var val := CaseMarshalling1.Parse(data[tagEnd..]);
+      value := Case1(val);
+    } else {
+      var val := CaseMarshalling2.Parse(data[tagEnd..]);
+      value := Case2(val);    
+    }
+  }
+
+  predicate marshallable(value: UnmarshalledType)
+  {
+    && TagMarshalling.Int.MinValue() <= 0 < 2 < TagMarshalling.Int.UpperBound()
+    && match value {
+      case Case0(c0) => CaseMarshalling0.marshallable(c0)
+      case Case1(c1) => CaseMarshalling1.marshallable(c1)
+      case Case2(c2) => CaseMarshalling2.marshallable(c2)
+    }
+  }
+
+  function size(value: UnmarshalledType) : nat
+  {
+    var tagEnd := getTagEnd();
+    match value {
+      case Case0(c0) => tagEnd as nat + CaseMarshalling0.size(c0)
+      case Case1(c1) => tagEnd as nat + CaseMarshalling1.size(c1)
+      case Case2(c2) => tagEnd as nat + CaseMarshalling2.size(c2)
+    }
+  }
+
+  method Size(value: UnmarshalledType) returns (sz: uint64)
+  {
+    sz := getTagEnd();
+    match value
+    case Case0(c0) => {
+      var size := CaseMarshalling0.Size(c0);
+      sz := sz + size;
+    }
+    case Case1(c1) => {
+      var size := CaseMarshalling1.Size(c1);
+      sz := sz + size;
+    }
+    case Case2(c2) => {
+      var size := CaseMarshalling2.Size(c2);
+      sz := sz + size;
+    }
+  }
+
+  method Marshall(value: UnmarshalledType, linear data: mseq<byte>, start: uint64)
+    returns (linear newdata: mseq<byte>, end: uint64)
+  {
+    ghost var tagEnd : uint64 := getTagEnd();
+
+    match value
+    case Case0(c0) => {
+      newdata, end := TagMarshalling.Marshall(TagMarshalling.Int.fromUint64(0), data, start);
+      ghost var newdata1 :seq<byte>, end1 := newdata, end;
+      newdata, end := CaseMarshalling0.Marshall(c0, newdata, end);
+
+      assert newdata1[start..end1] == newdata[start..end1];
+      ghost var tag := TagMarshalling.Int.toInt(TagMarshalling.parse(newdata[start..end1]));
+      TagMarshalling.Int.fromtoInverses();
+      assert tag == 0;
+
+      assert newdata[start..end][..tagEnd] == newdata[start..end1];
+    }
+    case Case1(c1) => {
+      newdata, end := TagMarshalling.Marshall(TagMarshalling.Int.fromUint64(1), data, start);
+      ghost var newdata1 :seq<byte>, end1 := newdata, end;
+      newdata, end := CaseMarshalling1.Marshall(c1, newdata, end);
+  
+      assert newdata1[start..end1] == newdata[start..end1];
+      ghost var tag := TagMarshalling.Int.toInt(TagMarshalling.parse(newdata[start..end1]));
+      TagMarshalling.Int.fromtoInverses();
+      assert tag == 1;
+
+      assert newdata[start..end][..tagEnd] == newdata[start..end1];
+    }
+    case Case2(c2) => {
+      newdata, end := TagMarshalling.Marshall(TagMarshalling.Int.fromUint64(2), data, start);
+      ghost var newdata1 :seq<byte>, end1 := newdata, end;
+      newdata, end := CaseMarshalling2.Marshall(c2, newdata, end);
+  
+      assert newdata1[start..end1] == newdata[start..end1];
+      ghost var tag := TagMarshalling.Int.toInt(TagMarshalling.parse(newdata[start..end1]));
+      TagMarshalling.Int.fromtoInverses();
+      assert tag == 2;
 
       assert newdata[start..end][..tagEnd] == newdata[start..end1];
     }
